MonadState.v
@@ -1,0 +1,150 @@
+
+Add LoadPath "." as PredMonad.
+Require Import PredMonad.Monad.
+
+
+(***
+ *** The State Monad
+ ***)
+
+(* StateT itself *)
+Definition StateT (S:Type) (M: Type -> Type) (X:Type) := S -> M (prod S X).
+
+Instance StateT_MonadOps S {LRS:LogRel_Rel S} `{MonadOps} : MonadOps (StateT S M) :=
+  {returnM :=
+     fun A x => fun s => returnM (s, x);
+   bindM :=
+     fun A B m f =>
+       fun s => bindM (m s) (fun (sx:S * A) => let (s',x) := sx in f x s');
+   equalsM :=
+     fun {A} {LR} m1 m2 => forall s, equalsM (m1 s) (m2 s) }.
+
+
+(* The Monad instance for StateT *)
+Instance StateT_Monad S `{LogRel S} `{Monad} : Monad (StateT S M).
+  constructor; simpl; intros.
+
+  intro; rewrite (monad_return_bind (M:=M));
+    [ reflexivity | auto with typeclass_instances ].
+
+  intro; transitivity (bindM (m s) returnM); [ | apply monad_bind_return ].
+  apply bind_fun_equalsM; intros.
+  intros p1 p2 ep; destruct p1; destruct p2.
+  apply monad_proper_return; [ auto with typeclass_instances | assumption ].
+  auto with typeclass_instances.
+  destruct x; reflexivity.
+  auto with typeclass_instances.
+
+FIXME HERE
+
+  intro; rewrite monad_assoc.
+  eapply bind_fun_equalsM. intro sx; destruct sx.
+  apply bind_fun_eqM; intro sx; destruct sx.
+  reflexivity.
+  split; intro; intros; intro; intros.
+  reflexivity.
+  symmetry; apply H0.
+  transitivity (y s); [ apply H0 | apply H1 ].
+  intros m1 m2 em f1 f2 ef s.
+  rewrite (em s).
+  apply bind_fun_eqM; intro sx; destruct sx.
+  apply ef; reflexivity.
+
+  constructor; constructor.
+  intros m s; reflexivity.
+  intros m1 m2 e s; symmetry; apply e.
+  intros m1 m2 m3 e1 e2 s; transitivity (m2 s); [ apply e1 | apply e2 ].
+
+  intros x y exy s. apply monad_proper_return.
+  auto with typeclass_instances.
+  split.
+  reflexivity.
+  assumption.
+
+Qed.
+
+
+(* The stateful computations class(es) *)
+
+Class MonadGet (S:Type) (M:Type -> Type) : Type := getM : M S.
+Class MonadPut (S:Type) (M:Type -> Type) : Type := putM : S -> M unit.
+
+Class MonadState S M {MonadRet:MonadRet M} {MonadBind:MonadBind M}
+      {MonadEquiv:MonadEquiv M} {MonadGet:MonadGet S M} {MonadPut:MonadPut S M}
+: Prop :=
+  {
+    monad_state_monad : @Monad M MonadRet MonadBind MonadEquiv;
+    monad_state_get_get :
+      forall A f,
+        bindM getM (fun s => bindM getM (f s)) ==
+        (bindM getM (fun s => f s s) : M A);
+    monad_state_get_put : bindM getM putM == returnM tt;
+    monad_state_put_get :
+      forall s, bindM (putM s) (fun _ => getM) ==
+                bindM (putM s) (fun _ => returnM s);
+    monad_state_put_put :
+      forall s1 s2, bindM (putM s1) (fun _ => putM s2) == putM s2
+  }.
+
+(* The MonadState instance for StateT *)
+
+Instance StateT_getM {S} `{MonadRet} : MonadGet S (StateT S M) :=
+  fun s => returnM (s, s).
+Instance StateT_putM {S} `{MonadRet} : MonadPut S (StateT S M) :=
+  fun s_new s => returnM (s_new, tt).
+
+Instance StateT_MonadState S `{Monad} : MonadState S (StateT S M).
+  constructor; intros; try apply StateT_Monad;
+    unfold returnM, StateT_returnM, bindM, StateT_bindM,
+           getM, StateT_getM, putM, StateT_putM; intros;
+    try (intros; intro; repeat (rewrite monad_return_bind); reflexivity).
+  assumption.
+Qed.
+
+
+FIXME HERE: move all the following to a new file, MonadFix.v
+
+(***
+ *** Non-Termination Effects
+ ***)
+
+(* approxM m1 m2 means m1 "approximates" m2, i.e., m2 is "at least as
+terminating as" m1 *)
+Class MonadApprox (M:Type -> Type) : Type :=
+  approxM : forall {A}, relation (M A).
+
+Notation "m1 '<<<' m2" := (approxM m1 m2) (at level 80, no associativity).
+
+Class MonadFixM (M:Type -> Type) : Type :=
+  fixM : forall {A B}, ((A -> M B) -> (A -> M B)) -> A -> M B.
+
+Class MonadFix M {MonadRet:MonadRet M} {MonadBind:MonadBind M}
+      {MonadEquiv:MonadEquiv M} {MonadApprox:MonadApprox M}
+      {MonadFixM:MonadFixM M}
+: Prop :=
+  {
+    monad_fix_monad :> @Monad M MonadRet MonadBind MonadEquiv;
+    monad_fix_approx_preorder :> forall A, PreOrder (approxM (A:=A));
+    monad_fix_approx_antisymmetry :
+      forall A (m1 m2:M A), approxM m1 m2 -> approxM m2 m1 -> m1 == m2;
+    monad_fix_approx_bind :>
+      forall A B,
+        Proper
+          (approxM (A:=A) ==> (@eq A ==> approxM (A:=B)) ==> approxM (A:=B))
+          bindM;
+    monad_fix_approx_proper :>
+      forall A, Proper (eqM (A:=A) ==> eqM (A:=A) ==> iff) approxM;
+    monad_fix_fix_proper :>
+      forall A B,
+        Proper (((@eq A ==> eqM (A:=B)) ==> @eq A ==> eqM (A:=B))
+                  ==> @eq A ==> eqM (A:=B)) fixM;
+    monad_fix_fixm :
+      forall A B f x,
+        Proper (((@eq A) ==> (approxM (A:=B))) ==> @eq A ==> approxM (A:=B)) f ->
+        fixM (A:=A) (B:=B) f x == f (fixM f) x
+  }.
+
+Add Parametric Relation `{MonadFix} A : (M A) (approxM (A:=A))
+  reflexivity proved by PreOrder_Reflexive
+  transitivity proved by PreOrder_Transitive
+as approxM_morphism.
